refactoring

coq/lib/P4cub/Transformations/Lifting/Lift.v
@@ -6,185 +6,185 @@ From Poulet4 Require Import
      P4cub.Syntax.IndPrincip
      P4cub.Transformations.Lifting.Statementize
      Utils.ForallMap.
-Import ListNotations AllCubNotations Nat.
+Import ListNotations Nat.
 From RecordUpdate Require Import RecordSet.
 Import RecordSetNotations.
 
-Local Open Scope expr_scope.
-Local Open Scope stmt_scope.
+Local Open Scope exp_scope.
+Local Open Scope stm_scope.
 
 Goal forall e es,
-    shift_pairs shift_e [(e,es)] = [(e,es)].
+    shift_pairs shift_exp [(e,es)] = [(e,es)].
 Proof.
-  intros; cbn; rewrite shift_e_0 , shift_elist_0. reflexivity.
+  intros; cbn; rewrite shift_exp_0 , shift_explist_0. reflexivity.
 Qed.
 
 Goal forall e1 e2 es1 es2,
-    shift_pairs shift_e [(e2,es2);(e1,es1)]
-    = [(shift_e (Shifter (length es2) (length es1)) e2,
-         shift_list shift_e (Shifter 0 (length es1)) es2);
-       (shift_e (Shifter 0 (length es2)) e1, es1)].
+    shift_pairs shift_exp [(e2,es2);(e1,es1)]
+    = [(shift_exp (Shifter (length es2) (length es1)) e2,
+         shift_list shift_exp (Shifter 0 (length es1)) es2);
+       (shift_exp (Shifter 0 (length es2)) e1, es1)].
 Proof.
   intros; unravel.
-  rewrite add_0_r, shift_elist_0, shift_e_0.
+  rewrite add_0_r, shift_explist_0, shift_exp_0.
   reflexivity.
 Qed.
 
 Goal forall e1 e2 e3 es1 es2 es3,
-    shift_pairs shift_e [(e3,es3);(e2,es2);(e1,es1)]
-    = [(shift_e (Shifter (length es3) (length es2 + length es1)) e3,
-            shift_list shift_e (Shifter 0 (length es2 + length es1)) es3);
-       (shift_e (Shifter 0 (length es3)) (shift_e (Shifter (length es2) (length es1)) e2),
-         shift_list shift_e (Shifter 0 (length es1)) es2);
-       (shift_e (Shifter 0 (length es3 + length es2)) e1, es1)].
+    shift_pairs shift_exp [(e3,es3);(e2,es2);(e1,es1)]
+    = [(shift_exp (Shifter (length es3) (length es2 + length es1)) e3,
+            shift_list shift_exp (Shifter 0 (length es2 + length es1)) es3);
+       (shift_exp (Shifter 0 (length es3)) (shift_exp (Shifter (length es2) (length es1)) e2),
+         shift_list shift_exp (Shifter 0 (length es1)) es2);
+       (shift_exp (Shifter 0 (length es3 + length es2)) e1, es1)].
 Proof.
   intros; unravel.
-  rewrite add_0_r, shift_elist_0, shift_e_0, shift_e_add.
+  rewrite add_0_r, shift_explist_0, shift_exp_0, shift_exp_add.
   reflexivity.
 Qed.
-       
-Inductive Lift_e
-  : Expr.e -> Expr.e -> list Expr.e -> Prop :=
+
+Inductive Lift_exp
+  : Exp.t -> Exp.t -> list Exp.t -> Prop :=
 | Lift_bool (b : bool) :
-  Lift_e b b []
+  Lift_exp (Exp.Bool b) (Exp.Bool b) []
 | Lift_var t og x :
-  Lift_e (Expr.Var t og x) (Expr.Var t og x) []
-| Lift_error err :
-  Lift_e (Expr.Error err) (Expr.Error err) []
+  Lift_exp (Exp.Var t og x) (Exp.Var t og x) []
+| Lift_exprror err :
+  Lift_exp (Exp.Error err) (Exp.Error err) []
 | Lift_bit w n :
-  Lift_e (w `W n) (Expr.Var (Expr.TBit w) "lifted_bit" 0) [w `W n]
+  Lift_exp (w `W n) (Exp.Var (Typ.Bit w) "lifted_bit" 0) [w `W n]
 | Lift_int w z :
-  Lift_e (w `S z) (Expr.Var (Expr.TInt w) "lifted_int" 0) [w `S z]
+  Lift_exp (w `S z) (Exp.Var (Typ.Int w) "lifted_int" 0) [w `S z]
 | Lift_varbit m w n :
-  Lift_e (Expr.VarBit m w n) (Expr.Var (Expr.TVarBit m) "lifted_varbit" 0) [Expr.VarBit m w n]
+  Lift_exp (Exp.VarBit m w n) (Exp.Var (Typ.VarBit m) "lifted_varbit" 0) [Exp.VarBit m w n]
 | Lift_member t x e e' es :
-  Lift_e e e' es ->
-  Lift_e (Expr.Member t x e) (Expr.Member t x e') es
+  Lift_exp e e' es ->
+  Lift_exp (Exp.Member t x e) (Exp.Member t x e') es
 | Lift_uop t o e e' es :
-  Lift_e e e' es ->
-  Lift_e (Expr.Uop t o e) (Expr.Var t "lifted_uop" 0) (Expr.Uop t o e' :: es)
+  Lift_exp e e' es ->
+  Lift_exp (Exp.Uop t o e) (Exp.Var t "lifted_uop" 0) (Exp.Uop t o e' :: es)
 | Lift_slice hi lo e e' es :
-  Lift_e e e' es ->
-  Lift_e
-    (Expr.Slice hi lo e)
-    (Expr.Var (Expr.TBit (Npos hi - Npos lo + 1)%N) "lifted_slice" 0)
-    (Expr.Slice hi lo e' :: es)
+  Lift_exp e e' es ->
+  Lift_exp
+    (Exp.Slice hi lo e)
+    (Exp.Var (Typ.Bit (Npos hi - Npos lo + 1)%N) "lifted_slice" 0)
+    (Exp.Slice hi lo e' :: es)
 | Lift_cast t e e' es :
-  Lift_e e e' es ->
-  Lift_e (Expr.Cast t e) (Expr.Var t "lifted_cast" 0) (Expr.Cast t e' :: es)
+  Lift_exp e e' es ->
+  Lift_exp (Exp.Cast t e) (Exp.Var t "lifted_cast" 0) (Exp.Cast t e' :: es)
 | Lift_index t e1 e2 e1' e2' es1 es2 :
-  Lift_e e1 e1' es1 ->
-  Lift_e e2 e2' es2 ->
-  Lift_e
-    (Expr.Index t e1 e2)
-    (Expr.Index
+  Lift_exp e1 e1' es1 ->
+  Lift_exp e2 e2' es2 ->
+  Lift_exp
+    (Exp.Index t e1 e2)
+    (Exp.Index
        t
-       (shift_e (Shifter 0 (length es2)) e1')
-       (shift_e (Shifter (length es2) (length es1)) e2'))
-    (shift_list shift_e (Shifter 0 (length es1)) es2 ++ es1)
+       (shift_exp (Shifter 0 (length es2)) e1')
+       (shift_exp (Shifter (length es2) (length es1)) e2'))
+    (shift_list shift_exp (Shifter 0 (length es1)) es2 ++ es1)
 | Lift_bop t o e1 e2 e1' e2' es1 es2 :
-  Lift_e e1 e1' es1 ->
-  Lift_e e2 e2' es2 ->
-  Lift_e
-    (Expr.Bop t o e1 e2)
-    (Expr.Var t "lifted_bop" 0)
-    (Expr.Bop
+  Lift_exp e1 e1' es1 ->
+  Lift_exp e2 e2' es2 ->
+  Lift_exp
+    (Exp.Bop t o e1 e2)
+    (Exp.Var t "lifted_bop" 0)
+    (Exp.Bop
        t o
-       (shift_e (Shifter 0 (length es2)) e1')
-       (shift_e (Shifter (length es2) (length es1)) e2')
-       :: shift_list shift_e (Shifter 0 (length es1)) es2 ++ es1)
+       (shift_exp (Shifter 0 (length es2)) e1')
+       (shift_exp (Shifter (length es2) (length es1)) e2')
+       :: shift_list shift_exp (Shifter 0 (length es1)) es2 ++ es1)
 | Lift_lists ls es es' ess :
-  Forall3 Lift_e es es' ess ->
-  Lift_e
-    (Expr.Lists ls es)
-    (Expr.Var (t_of_lists ls es) "lifted_lists" 0)
-    (Expr.Lists ls (map fst (shift_pairs shift_e (combine es' ess)))
-       :: concat (map snd (shift_pairs shift_e (combine es' ess)))).
+  Forall3 Lift_exp es es' ess ->
+  Lift_exp
+    (Exp.Lists ls es)
+    (Exp.Var (t_of_lists ls es) "lifted_lists" 0)
+    (Exp.Lists ls (map fst (shift_pairs shift_exp (combine es' ess)))
+       :: concat (map snd (shift_pairs shift_exp (combine es' ess)))).
 
 Section LifteInduction.
-  Variable P : Expr.e -> Expr.e -> list Expr.e -> Prop.
+  Variable P : Exp.t -> Exp.t -> list Exp.t -> Prop.
 
-  Hypothesis HLift_bool : forall (b : bool), P b b [].
+  Hypothesis HLift_bool : forall (b : bool), P (Exp.Bool b) (Exp.Bool b) [].
 
   Hypothesis HLift_var : forall t og x,
-      P (Expr.Var t og x) (Expr.Var t og x) [].
+      P (Exp.Var t og x) (Exp.Var t og x) [].
 
-  Hypothesis HLift_error : forall err,
-      P (Expr.Error err) (Expr.Error err) [].
+  Hypothesis HLift_exprror : forall err,
+      P (Exp.Error err) (Exp.Error err) [].
   
   Hypothesis HLift_bit : forall w n,
-      P (w `W n) (Expr.Var (Expr.TBit w) "lifted_bit" 0) [w `W n].
+      P (w `W n) (Exp.Var (Typ.Bit w) "lifted_bit" 0) [w `W n].
 
   Hypothesis HLift_int : forall w z,
-      P (w `S z) (Expr.Var (Expr.TInt w) "lifted_int" 0) [w `S z].
+      P (w `S z) (Exp.Var (Typ.Int w) "lifted_int" 0) [w `S z].
   
   Hypothesis HLift_varbit : forall m w n,
-      P (Expr.VarBit m w n) (Expr.Var (Expr.TVarBit m) "lifted_varbit" 0) [Expr.VarBit m w n].
+      P (Exp.VarBit m w n) (Exp.Var (Typ.VarBit m) "lifted_varbit" 0) [Exp.VarBit m w n].
 
   Hypothesis HLift_member : forall t x e e' es,
-      Lift_e e e' es ->
+      Lift_exp e e' es ->
       P e e' es ->
-      P (Expr.Member t x e) (Expr.Member t x e') es.
+      P (Exp.Member t x e) (Exp.Member t x e') es.
   
   Hypothesis HLift_uop : forall t o e e' es,
-      Lift_e e e' es ->
+      Lift_exp e e' es ->
       P e e' es ->
-      P (Expr.Uop t o e) (Expr.Var t "lifted_uop" 0) (Expr.Uop t o e' :: es).
+      P (Exp.Uop t o e) (Exp.Var t "lifted_uop" 0) (Exp.Uop t o e' :: es).
   
   Hypothesis HLift_slice : forall hi lo e e' es,
-      Lift_e e e' es ->
+      Lift_exp e e' es ->
       P e e' es ->
       P
-        (Expr.Slice hi lo e)
-        (Expr.Var (Expr.TBit (Npos hi - Npos lo + 1)%N) "lifted_slice" 0)
-        (Expr.Slice hi lo e' :: es).
+        (Exp.Slice hi lo e)
+        (Exp.Var (Typ.Bit (Npos hi - Npos lo + 1)%N) "lifted_slice" 0)
+        (Exp.Slice hi lo e' :: es).
   
   Hypothesis HLift_cast : forall t e e' es,
-      Lift_e e e' es ->
+      Lift_exp e e' es ->
       P e e' es ->
-      P (Expr.Cast t e) (Expr.Var t "lifted_cast" 0) (Expr.Cast t e' :: es).
+      P (Exp.Cast t e) (Exp.Var t "lifted_cast" 0) (Exp.Cast t e' :: es).
   
   Hypothesis HLift_index : forall t e1 e2 e1' e2' es1 es2,
-      Lift_e e1 e1' es1 ->
+      Lift_exp e1 e1' es1 ->
       P e1 e1' es1 ->
-      Lift_e e2 e2' es2 ->
+      Lift_exp e2 e2' es2 ->
       P e2 e2' es2 ->
       P
-        (Expr.Index t e1 e2)
-        (Expr.Index
+        (Exp.Index t e1 e2)
+        (Exp.Index
            t
-           (shift_e (Shifter 0 (length es2)) e1')
-           (shift_e (Shifter (length es2) (length es1)) e2'))
-        (shift_list shift_e (Shifter 0 (length es1)) es2 ++ es1).
+           (shift_exp (Shifter 0 (length es2)) e1')
+           (shift_exp (Shifter (length es2) (length es1)) e2'))
+        (shift_list shift_exp (Shifter 0 (length es1)) es2 ++ es1).
   
   Hypothesis HLift_bop : forall t o e1 e2 e1' e2' es1 es2,
-      Lift_e e1 e1' es1 ->
+      Lift_exp e1 e1' es1 ->
       P e1 e1' es1 ->
-      Lift_e e2 e2' es2 ->
+      Lift_exp e2 e2' es2 ->
       P e2 e2' es2 ->
       P
-        (Expr.Bop t o e1 e2)
-        (Expr.Var t "lifted_bop" 0)
-        (Expr.Bop
+        (Exp.Bop t o e1 e2)
+        (Exp.Var t "lifted_bop" 0)
+        (Exp.Bop
            t o
-           (shift_e (Shifter 0 (length es2)) e1')
-           (shift_e (Shifter (length es2) (length es1)) e2')
-           :: shift_list shift_e (Shifter 0 (length es1)) es2 ++ es1).
+           (shift_exp (Shifter 0 (length es2)) e1')
+           (shift_exp (Shifter (length es2) (length es1)) e2')
+           :: shift_list shift_exp (Shifter 0 (length es1)) es2 ++ es1).
   
   Hypothesis HLift_lists : forall ls es es' ess,
-      Forall3 Lift_e es es' ess ->
+      Forall3 Lift_exp es es' ess ->
       Forall3 P es es' ess ->
       P
-        (Expr.Lists ls es)
-        (Expr.Var (t_of_lists ls es) "lifted_lists" 0)
-        (Expr.Lists ls (map fst (shift_pairs shift_e (combine es' ess)))
-           :: concat (map snd (shift_pairs shift_e (combine es' ess)))).
+        (Exp.Lists ls es)
+        (Exp.Var (t_of_lists ls es) "lifted_lists" 0)
+        (Exp.Lists ls (map fst (shift_pairs shift_exp (combine es' ess)))
+           :: concat (map snd (shift_pairs shift_exp (combine es' ess)))).
 
-  Definition custom_Lift_e_ind : forall e e' es,
-      Lift_e e e' es -> P e e' es :=
+  Definition custom_Lift_exp_ind : forall e e' es,
+      Lift_exp e e' es -> P e e' es :=
     fix F e e' es hLift :=
-      let fix F3 {es es' : list Expr.e} {ess : list (list Expr.e)}
-            (h : Forall3 Lift_e es es' ess)
+      let fix F3 {es es' : list Exp.t} {ess : list (list Exp.t)}
+            (h : Forall3 Lift_exp es es' ess)
         : Forall3 P es es' ess :=
         match h with
         | Forall3_nil _ => Forall3_nil _
@@ -194,7 +194,7 @@ Section LifteInduction.
       match hLift with
       | Lift_bool b => HLift_bool b
       | Lift_var x y z => HLift_var x y z
-      | Lift_error e => HLift_error e
+      | Lift_exprror e => HLift_exprror e
       | Lift_bit x y => HLift_bit x y
       | Lift_int x y => HLift_int x y
       | Lift_varbit m x y => HLift_varbit m x y
@@ -211,131 +211,126 @@ Section LifteInduction.
 End LifteInduction.
 
 Variant Lift_arg :
-  Expr.arg -> Expr.arg -> list Expr.e -> Prop :=
+  Exp.arg -> Exp.arg -> list Exp.t -> Prop :=
   | Lift_pain e e' es :
-    Lift_e e e' es ->
+    Lift_exp e e' es ->
     Lift_arg (PAIn e) (PAIn e') es
   | Lift_paout e e' es :
-    Lift_e e e' es ->
+    Lift_exp e e' es ->
     Lift_arg (PAOut e) (PAOut e') es
   | Lift_painout e e' es :
-    Lift_e e e' es ->
+    Lift_exp e e' es ->
     Lift_arg (PAInOut e) (PAInOut e') es.
 
-Variant Lift_trans :
-  Parser.trns -> Parser.trns -> list Expr.e ->  Prop :=
+Variant Lift_trns :
+  Trns.t -> Trns.t -> list Exp.t ->  Prop :=
   | Lift_direct lbl :
-    Lift_trans (Parser.Direct lbl) (Parser.Direct lbl) []
+    Lift_trns (Trns.Direct lbl) (Trns.Direct lbl) []
   | Lift_select e e' es d cases :
-    Lift_e e e' es ->
-    Lift_trans
-      (Parser.Select e d cases)
-      (Parser.Select e' d cases) es.
+    Lift_exp e e' es ->
+    Lift_trns
+      (Trns.Select e d cases)
+      (Trns.Select e' d cases) es.
 
-Variant Lift_fun_kind :
-  Stmt.fun_kind -> Stmt.fun_kind -> list Expr.e -> Prop :=
+Variant Lift_call :
+  Call.t -> Call.t -> list Exp.t -> Prop :=
   | Lift_funct_none f τs :
-    Lift_fun_kind (Stmt.Funct f τs None) (Stmt.Funct f τs None) []
+    Lift_call (Call.Funct f τs None) (Call.Funct f τs None) []
   | Lift_method_none ext mtd τs :
-    Lift_fun_kind
-      (Stmt.Method ext mtd τs None)
-      (Stmt.Method ext mtd τs None) []
+    Lift_call
+      (Call.Method ext mtd τs None)
+      (Call.Method ext mtd τs None) []
   | Lift_funct_some f τs e e' es :
-    Lift_e e e' es ->
-    Lift_fun_kind
-      (Stmt.Funct f τs (Some e))
-      (Stmt.Funct f τs (Some e')) es
+    Lift_exp e e' es ->
+    Lift_call
+      (Call.Funct f τs (Some e))
+      (Call.Funct f τs (Some e')) es
   | Lift_method_some ext mtd τs e e' es :
-    Lift_e e e' es ->
-    Lift_fun_kind
-      (Stmt.Method ext mtd τs (Some e))
-      (Stmt.Method ext mtd τs (Some e')) es
+    Lift_exp e e' es ->
+    Lift_call
+      (Call.Method ext mtd τs (Some e))
+      (Call.Method ext mtd τs (Some e')) es
   | Lift_action_call a cargs cargs' ess :
-    Forall3 Lift_e cargs cargs' ess ->
-    Lift_fun_kind
-      (Stmt.Action a cargs)
-      (Stmt.Action a (map fst (shift_pairs shift_e (combine cargs' ess))))
-      (concat (map snd (shift_pairs shift_e (combine cargs' ess)))).
+    Forall3 Lift_exp cargs cargs' ess ->
+    Lift_call
+      (Call.Action a cargs)
+      (Call.Action a (map fst (shift_pairs shift_exp (combine cargs' ess))))
+      (concat (map snd (shift_pairs shift_exp (combine cargs' ess))))
+  | Lift_inst_call x eargs :
+    Lift_call (Call.Inst x eargs) (Call.Inst x eargs) [].
 
-Inductive Lift_s : Stmt.s -> Stmt.s -> Prop :=
-| Lift_skip :
-  Lift_s Stmt.Skip Stmt.Skip
+Inductive Lift_stm : Stm.t -> Stm.t -> Prop :=
+| Lift_stmkip :
+  Lift_stm Stm.Skip Stm.Skip
 | Lift_exit :
-  Lift_s Stmt.Exit Stmt.Exit
+  Lift_stm Stm.Exit Stm.Exit
 | Lift_return_none :
-  Lift_s (Stmt.Return None) (Stmt.Return None)
+  Lift_stm (Stm.Ret None) (Stm.Ret None)
 | Lift_return_some e e' es :
-  Lift_e e e' es ->
-  Lift_s
-    (Stmt.Return (Some e))
-    (Unwind es (Stmt.Return (Some e')))
+  Lift_exp e e' es ->
+  Lift_stm
+    (Stm.Ret (Some e))
+    (Unwind es (Stm.Ret (Some e')))
 | Lift_transition e e' es :
-  Lift_trans e e' es ->
-  Lift_s
-    (Stmt.Transition e)
-    (Unwind es (Stmt.Transition e'))
+  Lift_trns e e' es ->
+  Lift_stm
+    (Stm.Trans e)
+    (Unwind es (Stm.Trans e'))
 | Lift_asgn e1 e2 e1' e2' es1 es2 :
-  Lift_e e1 e1' es1 ->
-  Lift_e e2 e2' es2 ->
-  Lift_s
+  Lift_exp e1 e1' es1 ->
+  Lift_exp e2 e2' es2 ->
+  Lift_stm
     (e1 `:= e2)
     (Unwind
-       (shift_list shift_e (Shifter 0 (length es1)) es2 ++ es1)
-       (shift_e (Shifter 0 (length es2)) e1'
-          `:= shift_e (Shifter (length es2) (length es1)) e2'))
+       (shift_list shift_exp (Shifter 0 (length es1)) es2 ++ es1)
+       (shift_exp (Shifter 0 (length es2)) e1'
+          `:= shift_exp (Shifter (length es2) (length es1)) e2'))
 | Lift_invoke_none t :
-  Lift_s (Stmt.Invoke None t) (Stmt.Invoke None t)
+  Lift_stm (Stm.Invoke None t) (Stm.Invoke None t)
 | Lift_invoke e e' t es :
-  Lift_e e e' es ->
-  Lift_s
-    (Stmt.Invoke (Some e) t)
-    (Unwind es (Stmt.Invoke (Some e') t))
-| Lift_call fk fk' fkes args args' argsess :
-  Lift_fun_kind fk fk' fkes ->
+  Lift_exp e e' es ->
+  Lift_stm
+    (Stm.Invoke (Some e) t)
+    (Unwind es (Stm.Invoke (Some e') t))
+| Lift_app fk fk' fkes args args' argsess :
+  Lift_call fk fk' fkes ->
   Forall3 Lift_arg args args' argsess ->
-  Lift_s
-    (Stmt.Call fk args)
+  Lift_stm
+    (Stm.App fk args)
     (Unwind
-       (shift_list shift_e (Shifter 0 (length (concat argsess))) fkes
+       (shift_list shift_exp (Shifter 0 (length (concat argsess))) fkes
           ++ concat (map snd (shift_pairs shift_arg (combine args' argsess))))
-       (Stmt.Call
-           (shift_fun_kind (Shifter (length fkes) (length (concat argsess))) fk')
+       (Stm.App
+           (shift_call (Shifter (length fkes) (length (concat argsess))) fk')
            (map (shift_arg $ Shifter 0 (length fkes))
               (map fst (shift_pairs shift_arg (combine args' argsess))))))
-| Lift_apply x exts args args' argsess :
-  Forall3 Lift_arg args args' argsess ->
-  Lift_s
-    (Stmt.Apply x exts args)
-    (Unwind
-       (concat (map snd (shift_pairs shift_arg (combine args' argsess))))
-       (Stmt.Apply x exts
-          (map fst (shift_pairs shift_arg (combine args' argsess)))))
-| Lift_seq s1 s2 s1' s2' :
-  Lift_s s1 s1' ->
-  Lift_s s2 s2' ->
-  Lift_s (s1 `; s2) (s1' `; s2')
+| Lift_stmeq s1 s2 s1' s2' :
+  Lift_stm s1 s1' ->
+  Lift_stm s2 s2' ->
+  Lift_stm (s1 `; s2) (s1' `; s2')
 | Lift_if e e' s1 s2 s1' s2' es :
-  Lift_e e e' es ->
-  Lift_s s1 s1' ->
-  Lift_s s2 s2' ->
-  Lift_s
-    (If e Then s1 Else s2)
+  Lift_exp e e' es ->
+  Lift_stm s1 s1' ->
+  Lift_stm s2 s2' ->
+  Lift_stm
+    (`if e `then s1 `else s2)
     (Unwind
        es
-       (If e'
-          Then shift_s (Shifter 0 (length es)) s1'
-          Else shift_s (Shifter 0 (length es)) s2'))
+       (`if e'
+          `then shift_stm (Shifter 0 (length es)) s1'
+          `else shift_stm (Shifter 0 (length es)) s2'))
 | Lift_var_typ og t s s' :
-  Lift_s s s' ->
-  Lift_s (Stmt.Var og (inl t) s) (Stmt.Var og (inl t) s')
+  Lift_stm s s' ->
+  Lift_stm
+    (`let og := inl t `in s) (`let og := inl t `in s')
 | Lift_var_exp og e e' s s' es :
-  Lift_e e e' es ->
-  Lift_s s s' ->
-  Lift_s
-    (Stmt.Var og (inr e) s)
+  Lift_exp e e' es ->
+  Lift_stm s s' ->
+  Lift_stm
+    (`let og := inr e `in s)
     (Unwind
        es
-       (Stmt.Var og (inr e') (shift_s (Shifter 1 (length es)) s'))).
+       (`let og := inr e' `in shift_stm (Shifter 1 (length es)) s')).
 
 Ltac destr_call_pair f :=
   match goal with
@@ -343,36 +338,36 @@ Ltac destr_call_pair f :=
     => destruct (f a) as [? ?] eqn:?; subst
   end.
     
-Ltac destr_lift_e := destr_call_pair lift_e.
+Ltac destr_lift_exp := destr_call_pair lift_exp.
 
 Ltac destr_lift_arg := destr_call_pair lift_arg.
 
-Ltac destr_lift_e_list := destr_call_pair lift_e_list.
+Ltac destr_lift_exp_list := destr_call_pair lift_exp_list.
 
-Ltac destr_lift_trans := destr_call_pair lift_trans.
+Ltac destr_lift_trns := destr_call_pair lift_trns.
 
 Ltac destr_lift_args := destr_call_pair lift_args.
 
 Section Liftlift.
-  Lemma Lift_lift_e : forall e e' es,
-      Lift_e e e' es -> lift_e e = (e', es).
+  Lemma Lift_lift_exp : forall e e' es,
+      Lift_exp e e' es -> lift_exp e = (e', es).
   Proof.
     intros e e' es h;
-      induction h using custom_Lift_e_ind;
+      induction h using custom_Lift_exp_ind;
       unravel;
-      repeat destr_lift_e;
+      repeat destr_lift_exp;
       repeat match goal with
         | h: (_, _) = (_, _) |- _ => inv h
         end; auto.
-    destruct (split (shift_pairs shift_e (map lift_e es)))
+    destruct (split (shift_pairs shift_exp (map lift_exp es)))
       as [es'' les] eqn:hsplit.
     rewrite split_map in hsplit. inv hsplit.
-    enough (map lift_e es = combine es' ess) as h.
+    enough (map lift_exp es = combine es' ess) as h.
     { do 5 f_equal; assumption. }
     assert (h12 : length es = length es') by eauto using Forall3_length12.
     rewrite Forall3_map_1 with
       (R:=fun e e' es => e = (e', es))
-      (f:=lift_e) in H0.
+      (f:=lift_exp) in H0.
     rewrite Forall3_Forall2_combine_r in H0.
     destruct H0 as [_ h].
     rewrite <- Forall2_eq.
@@ -383,15 +378,15 @@ Section Liftlift.
     firstorder.
   Qed.
 
-  Local Hint Resolve Lift_lift_e : core.
+  Local Hint Resolve Lift_lift_exp : core.
 
-  Ltac apply_Lift_lift_e :=
+  Ltac apply_Lift_lift_exp :=
     match goal with
-    | h: Lift_e _ _ _
-      |- _ => apply Lift_lift_e in h; rewrite h
+    | h: Lift_exp _ _ _
+      |- _ => apply Lift_lift_exp in h; rewrite h
     end.
 
-  Local Hint Extern 5 => apply_Lift_lift_e : core.
+  Local Hint Extern 5 => apply_Lift_lift_exp : core.
 
   Lemma Lift_lift_arg : forall arg arg' es,
       Lift_arg arg arg' es ->
@@ -410,60 +405,60 @@ Section Liftlift.
   
   Local Hint Extern 5 => apply_Lift_lift_arg : core.
 
-  Lemma Lift_lift_trans : forall pe pe' es,
-      Lift_trans pe pe' es ->
-      lift_trans pe = (pe',es).
+  Lemma Lift_lift_trns : forall pe pe' es,
+      Lift_trns pe pe' es ->
+      lift_trns pe = (pe',es).
   Proof.
     intros pe pe' es h; inv h; unravel; auto.
   Qed.
 
-  Local Hint Resolve Lift_lift_trans : core.
+  Local Hint Resolve Lift_lift_trns : core.
   
-  Ltac apply_Lift_lift_trans :=
+  Ltac apply_Lift_lift_trns :=
       match goal with
-      | h: Lift_trans _ _ _
-        |- _ => apply Lift_lift_trans in h; rewrite h
+      | h: Lift_trns _ _ _
+        |- _ => apply Lift_lift_trns in h; rewrite h
       end.
 
-  Local Hint Extern 5 => apply_Lift_lift_trans : core.
+  Local Hint Extern 5 => apply_Lift_lift_trns : core.
 
-  Lemma Forall3_Lift_lift_e : forall es es' ess,
-      Forall3 Lift_e es es' ess ->
-      map lift_e es = combine es' ess.
+  Lemma Forall3_Lift_lift_exp : forall es es' ess,
+      Forall3 Lift_exp es es' ess ->
+      map lift_exp es = combine es' ess.
   Proof.
     intros es es' ess h;
       induction h; cbn; f_equal; auto.
   Qed.
 
-  Ltac apply_Forall3_Lift_lift_e :=
+  Ltac apply_Forall3_Lift_lift_exp :=
     match goal with
-    | h : Forall3 Lift_e _ _ _
-      |- _ => apply Forall3_Lift_lift_e in h; rewrite h
+    | h : Forall3 Lift_exp _ _ _
+      |- _ => apply Forall3_Lift_lift_exp in h; rewrite h
     end.
 
-  Local Hint Extern 5 => apply_Forall3_Lift_lift_e : core.
+  Local Hint Extern 5 => apply_Forall3_Lift_lift_exp : core.
   
-  Lemma Lift_lift_fun_kind : forall fk fk' es,
-      Lift_fun_kind fk fk' es ->
-      lift_fun_kind fk = (fk', es).
+  Lemma Lift_lift_call : forall fk fk' es,
+      Lift_call fk fk' es ->
+      lift_call fk = (fk', es).
   Proof.
     intros fk fk' es h; inv h; unravel; auto.
-    unfold lift_e_list.
-    destruct (split (shift_pairs shift_e $ map lift_e cargs))
+    unfold lift_exp_list.
+    destruct (split (shift_pairs shift_exp $ map lift_exp cargs))
       as [es les] eqn:hs.
     rewrite split_map in hs; unravel in hs; inv hs.
     auto.
   Qed.
 
-  Local Hint Resolve Lift_lift_fun_kind : core.
+  Local Hint Resolve Lift_lift_call : core.
 
-  Ltac apply_Lift_lift_fun_kind :=
+  Ltac apply_Lift_lift_call :=
       match goal with
-      | h: Lift_fun_kind _ _ _
-        |- _ => apply Lift_lift_fun_kind in h; rewrite h
+      | h: Lift_call _ _ _
+        |- _ => apply Lift_lift_call in h; rewrite h
       end.
 
-  Local Hint Extern 5 => apply_Lift_lift_fun_kind : core.
+  Local Hint Extern 5 => apply_Lift_lift_call : core.
   
   Lemma Forall3_Lift_lift_arg : forall args args' ess,
       Forall3 Lift_arg args args' ess ->
@@ -481,11 +476,11 @@ Section Liftlift.
 
   Local Hint Extern 5 => apply_Forall3_Lift_lift_arg : core.
 
-  Lemma Lift_lift_s : forall s s',
-      Lift_s s s' -> lift_s s = s'.
+  Lemma Lift_lift_stm : forall s s',
+      Lift_stm s s' -> lift_stm s = s'.
   Proof.
     intros s s' h; induction h; unravel; subst; auto.
-    - apply_Lift_lift_fun_kind.
+    - apply_Lift_lift_call.
       unfold lift_args.
       destruct
         (split (shift_pairs shift_arg $ map lift_arg args))
@@ -503,39 +498,33 @@ Section Liftlift.
         by eauto using Forall3_length23.
       apply_Forall3_Lift_lift_arg.
       repeat f_equal; auto using map_snd_combine.
-    - unfold lift_args.
-      destruct
-        (split (shift_pairs shift_arg $ map lift_arg args))
-        as [Args les] eqn:hsplit.
-      rewrite split_map in hsplit.
-      unravel in *; inv hsplit. auto.
   Qed.
 End Liftlift.
 
 Section liftLift.
-  Local Hint Constructors Lift_e : core.
+  Local Hint Constructors Lift_exp : core.
   
-  Lemma lift_Lift_e : forall e,
-    Lift_e e (fst (lift_e e)) (snd (lift_e e)).
+  Lemma lift_Lift_exp : forall e,
+    Lift_exp e (fst (lift_exp e)) (snd (lift_exp e)).
   Proof.
-    intro e; induction e using custom_e_ind; cbn;
-      repeat destr_lift_e; cbn in *; auto.
+    intro e; induction e using custom_exp_ind; cbn;
+      repeat destr_lift_exp; cbn in *; auto.
     - constructor. assumption.
     - destruct
-        (split (shift_pairs shift_e $ map lift_e exps)) as [es' les] eqn:hes.
+        (split (shift_pairs shift_exp $ map lift_exp es)) as [es' les] eqn:hes.
       rewrite split_map in hes.
       unravel in *. inv hes.
       assert (h: Forall3
-                   Lift_e
-                   exps
-                   (map fst (map lift_e exps))
-                   (map snd (map lift_e exps))).
+                   Lift_exp
+                   es
+                   (map fst (map lift_exp es))
+                   (map snd (map lift_exp es))).
       { clear l.
         rewrite Forall_forall in H.
         rewrite Forall3_forall.
         repeat rewrite map_length.
         repeat split; try reflexivity.
-        intros n e e' es he he' hes.
+        intros n e e' exps he he' hes.
         pose proof H _ (nth_error_In _ _ he) as h.
         do 2 rewrite nth_error_map in he',hes.
         rewrite he in he',hes.
@@ -543,30 +532,30 @@ Section liftLift.
         inv he'; inv hes.
         assumption. }
       rewrite <- combine_map_fst_snd
-        with (l:=map lift_e exps). auto.
+        with (l:=map lift_exp es). auto.
   Qed.
 
-  Local Hint Resolve lift_Lift_e : core.
+  Local Hint Resolve lift_Lift_exp : core.
 
   Ltac solve_aux h :=
     pose proof f_equal fst h as h1;
     pose proof f_equal snd h as h2;
     cbn in *; subst; auto.
   
-  Corollary lift_Lift_e_aux : forall e e' es,
-      lift_e e = (e', es) -> Lift_e e e' es.
+  Corollary lift_Lift_exp_aux : forall e e' es,
+      lift_exp e = (e', es) -> Lift_exp e e' es.
   Proof.
     intros e e' es h; solve_aux h.
   Qed.
 
-  Local Hint Resolve lift_Lift_e_aux : core.
+  Local Hint Resolve lift_Lift_exp_aux : core.
   Local Hint Constructors Lift_arg : core.
   
   Lemma lift_Lift_arg : forall arg,
       Lift_arg arg (fst (lift_arg arg)) (snd (lift_arg arg)).
   Proof.
     intros [e | e | e]; unravel;
-      destr_lift_e; cbn; auto.
+      destr_lift_exp; cbn; auto.
   Qed.
 
   Local Hint Resolve lift_Lift_arg : core.
@@ -579,41 +568,41 @@ Section liftLift.
   Qed.
 
   Local Hint Resolve lift_Lift_arg_aux : core.
-  Local Hint Constructors Lift_trans : core.
+  Local Hint Constructors Lift_trns : core.
   
-  Lemma lift_Lift_trans : forall e,
-      Lift_trans e (fst (lift_trans e)) (snd (lift_trans e)).
+  Lemma lift_Lift_trns : forall e,
+      Lift_trns e (fst (lift_trns e)) (snd (lift_trns e)).
   Proof.
     intros []; unravel;
-      try destr_lift_e; cbn; auto.
+      try destr_lift_exp; cbn; auto.
   Qed.
 
-  Local Hint Resolve lift_Lift_trans : core.
+  Local Hint Resolve lift_Lift_trns : core.
 
-  Corollary lift_Lift_trans_aux : forall e e' es,
-      lift_trans e = (e', es) ->
-      Lift_trans e e' es.
+  Corollary lift_Lift_trns_aux : forall e e' es,
+      lift_trns e = (e', es) ->
+      Lift_trns e e' es.
   Proof.
     intros e e' es h; solve_aux h.
   Qed.
 
-  Local Hint Resolve lift_Lift_trans_aux : core.
-  Local Hint Constructors Lift_fun_kind : core.
+  Local Hint Resolve lift_Lift_trns_aux : core.
+  Local Hint Constructors Lift_call : core.
 
-  Lemma lift_Lift_fun_kind : forall fk,
-      Lift_fun_kind fk (fst (lift_fun_kind fk)) (snd (lift_fun_kind fk)).
+  Lemma lift_Lift_call : forall fk,
+      Lift_call fk (fst (lift_call fk)) (snd (lift_call fk)).
   Proof.
-    intros [f ts [e |] | a cs | extrn mthd ts [e |]];
-      unravel; try destr_lift_e; cbn; auto.
-    destr_lift_e_list.
-    unfold lift_e_list in Heqp.
-    destruct (split (shift_pairs shift_e $ map lift_e cs))
+    intros [f ts [e |] | a cs | extrn mthd ts [e |] | ? ?];
+      unravel; try destr_lift_exp; cbn; auto.
+    destr_lift_exp_list.
+    unfold lift_exp_list in Heqp.
+    destruct (split (shift_pairs shift_exp $ map lift_exp cs))
       as [es ees] eqn:hsplit.
     unravel in *.
     rewrite split_map in hsplit.
     inv hsplit; inv Heqp.
     rewrite <- combine_map_fst_snd
-      with (l:=map lift_e cs).
+      with (l:=map lift_exp cs).
     constructor.
     rewrite Forall3_forall.
     repeat rewrite map_length.
@@ -624,29 +613,29 @@ Section liftLift.
     inv he'; inv hes. auto.
   Qed.
 
-  Local Hint Resolve lift_Lift_fun_kind : core.
+  Local Hint Resolve lift_Lift_call : core.
 
-  Lemma lift_Lift_fun_kind_aux : forall fk fk' es,
-      lift_fun_kind fk = (fk', es) ->
-      Lift_fun_kind fk fk' es.
+  Lemma lift_Lift_call_aux : forall fk fk' es,
+      lift_call fk = (fk', es) ->
+      Lift_call fk fk' es.
   Proof.
     intros fk fk' es h. solve_aux h.
   Qed.
 
-  Local Hint Resolve lift_Lift_fun_kind_aux : core.
-  Local Hint Constructors Lift_s : core.
+  Local Hint Resolve lift_Lift_call_aux : core.
+  Local Hint Constructors Lift_stm : core.
 
-  Lemma lift_Lift_stmt : forall s,
-      Lift_s s (lift_s s).
+  Lemma lift_Lift_stm : forall s,
+      Lift_stm s (lift_stm s).
   Proof.
     intro s; induction s; unravel;
-      try destr_lift_trans;
-      repeat destr_lift_e;
-      try destr_call_pair lift_fun_kind;
+      try destr_lift_trns;
+      repeat destr_lift_exp;
+      try destr_call_pair lift_call;
       try destr_lift_args;
       auto.
     - destruct e as [e |];
-        try destr_lift_e; auto.
+        try destr_lift_exp; auto.
     - unfold lift_args in Heqp0.
       destruct (split (shift_pairs shift_arg $ map lift_arg args))
         as [args' les] eqn:hsplit.
@@ -666,30 +655,12 @@ Section liftLift.
       repeat (split; try reflexivity).
       intros n arg arg' es harg harg' hes.
       do 2 rewrite nth_error_map in harg',hes.
-      unfold Expr.arg in *.
+      unfold Exp.arg in *.
       rewrite harg in harg',hes; cbn in *.
       inv harg'; inv hes. auto.
     - destruct lhs as [e |];
-        try destr_lift_e; eauto.
-    - unfold lift_args in Heqp.
-      destruct
-        (split (shift_pairs shift_arg $ map lift_arg args))
-        as [args' es] eqn:hsplit.
-      rewrite split_map in hsplit.
-      unravel in *.
-      inv hsplit; inv Heqp.
-      rewrite <- combine_map_fst_snd
-        with (l := map lift_arg args).
-      constructor.
-      rewrite Forall3_forall.
-      repeat rewrite map_length.
-      repeat (split; try reflexivity).
-      intros n arg arg' es harg harg' hes.
-      do 2 rewrite nth_error_map in harg',hes.
-      unfold Expr.arg in *.
-      rewrite harg in harg',hes; cbn in *.
-      inv harg'; inv hes. auto.
-    - destruct expr as [t | e];
-        try destr_lift_e; auto.
+        try destr_lift_exp; eauto.
+    - destruct init as [t | e];
+        try destr_lift_exp; auto.
   Qed.
 End liftLift.
