coq/lib/P4cub/Semantics/Denotation/Denote.v
@@ -1,5 +1,4 @@
 Require Export Poulet4.P4cub.Syntax.Syntax.
-Import AllCubNotations String.
 
 Fixpoint denote_list (l : list Set) : Set :=
   match l with
@@ -8,16 +7,18 @@ Fixpoint denote_list (l : list Set) : Set :=
   end.
 
 (* TODO: some denotations are  incomplete. *)
-Fail Fixpoint denote_t (t : Expr.t) : Set :=
-  let fix denote_ts (ts : list Expr.t) : Set :=
+Fail Fixpoint denote_typ (t : Typ.t) : Set :=
+  let fix denote_typs (ts : list Typ.t) : Set :=
       match ts with
       | []     => unit
-      | t :: ts => (denote_t t * denote_ts ts)%type
+      | t :: ts => (denote_typ t * denote_typs ts)%type
       end in
   match t with
-  | Expr.TBool => bool
-  | Expr.TBit _ => N
-  | Expr.TInt _ => Z
-  | Expr.TError => string
-  | Expr.TStruct ts _ => denote_ts ts
+  | Typ.Bool => bool
+  | Typ.Bit _ => N
+  | Typ.Int _ => Z
+  | Typ.Error => String.string
+  | Typ.Struct ts _ => denote_typs ts
+  | Typ.VarBit _ => N
+  | Typ.Array _ t => list $ denote_typ t
   end.
