coq/lib/P4cub/Syntax/Auxiliary.v
@@ -3,23 +3,22 @@ Require Import Coq.PArith.BinPos
         Coq.NArith.BinNat.
 From Poulet4 Require Import Utils.P4Arith
      P4cub.Syntax.AST P4cub.Syntax.CubNotations.
-Import Expr ExprNotations.
 
-Definition stmt_of_list : list Stmt.s -> Stmt.s :=
-  List.fold_right Stmt.Seq Stmt.Skip.
+Definition stmt_of_list : list Stm.t -> Stm.t :=
+  List.fold_right Stm.Seq Stm.Skip.
 
-Fixpoint width_of_typ (τ : t) : option nat :=
+Fixpoint width_of_typ (τ : Typ.t) : option nat :=
   match τ with
-  | TBool  => Some 1%nat
-  | TBit w => Some $ N.to_nat w
-  | TInt w => Some $ Pos.to_nat w
-  | TVarBit w => Some $ N.to_nat w
-  | TError => Some 0%nat
-  | TVar _ => None
-  | TArray n t =>
+  | Typ.Bool  => Some 1%nat
+  | Typ.Bit w => Some $ N.to_nat w
+  | Typ.Int w => Some $ Pos.to_nat w
+  | Typ.VarBit w => Some $ N.to_nat w
+  | Typ.Error => Some 0%nat
+  | Typ.Var _ => None
+  | Typ.Array n t =>
       width_of_typ
         t >>| mult $ N.to_nat n
-  | TStruct b fs =>
+  | Typ.Struct b fs =>
       sequence
         $ List.map width_of_typ fs
         >>| List.fold_right Nat.add 0%nat
@@ -27,28 +26,28 @@ Fixpoint width_of_typ (τ : t) : option nat :=
   end.
 
 (** Syntactic type of an expression. *)
-Fixpoint t_of_e (exp: e) : t := 
+Fixpoint t_of_e (exp: Exp.t) : Typ.t := 
   match exp with
-  | Bool _  => TBool
-  | Error _ => TError
-  | Var τ _ _
-  | Cast τ _
-  | Uop τ _ _
-  | Bop τ _ _ _
-  | Index τ _ _
-  | Member τ _ _  => τ
-  | (w `W _)%expr => TBit w
-  | (w `S _)%expr => TInt w
-  | VarBit m w _    => TVarBit m
-  | Slice hi lo _ => TBit (Npos hi - Npos lo + 1)%N
-  | Lists (lists_array τ) es  => TArray (N.of_nat $ List.length es) τ
-  | Lists lists_struct es     => TStruct false (List.map t_of_e es)
-  | Lists (lists_header _) es => TStruct true (List.map t_of_e es)
+  | Exp.Bool _  => Typ.Bool
+  | Exp.Error _ => Typ.Error
+  | Exp.Var τ _ _
+  | Exp.Cast τ _
+  | Exp.Uop τ _ _
+  | Exp.Bop τ _ _ _
+  | Exp.Index τ _ _
+  | Exp.Member τ _ _  => τ
+  | (w `W _)%exp => Typ.Bit w
+  | (w `S _)%exp => Typ.Int w
+  | Exp.VarBit m w _    => Typ.VarBit m
+  | Exp.Slice hi lo _ => Typ.Bit (Npos hi - Npos lo + 1)%N
+  | Exp.Lists (Lst.Array τ) es  => Typ.Array (N.of_nat $ List.length es) τ
+  | Exp.Lists Lst.Struct es     => Typ.Struct false (List.map t_of_e es)
+  | Exp.Lists (Lst.Header _) es => Typ.Struct true (List.map t_of_e es)
   end.
 
-Definition t_of_lists (ls : Expr.lists) (es : list Expr.e) : Expr.t :=
+Definition t_of_lists (ls : Lst.t) (es : list Exp.t) : Typ.t :=
   match ls with
-  | lists_array t  => TArray (N.of_nat $ List.length es) t
-  | lists_struct   => TStruct false (List.map t_of_e es)
-  | lists_header _ => TStruct true (List.map t_of_e es)
+  | Lst.Array t  => Typ.Array (N.of_nat $ List.length es) t
+  | Lst.Struct   => Typ.Struct false (List.map t_of_e es)
+  | Lst.Header _ => Typ.Struct true (List.map t_of_e es)
   end.
